lean/Brainfuck/Program/ValidatedProgram.lean
@@ -5,6 +5,7 @@ namespace Brainfuck.Program
 open Brainfuck.Core
 
 abbrev ProgramIndex (length : Nat) := Fin length
+abbrev ProgramCounter (length : Nat) := Fin (length + 1)
 
 inductive ValidatedInstruction (length : Nat) where
   | moveRight
@@ -13,14 +14,14 @@ inductive ValidatedInstruction (length : Nat) where
   | decrement
   | output
   | input
-  | jumpIfZero (target : ProgramIndex length)
-  | jumpIfNonZero (target : ProgramIndex length)
-  deriving Repr
+  | jumpIfZero (target : ProgramCounter length)
+  | jumpIfNonZero (target : ProgramCounter length)
+  deriving DecidableEq, Repr
 
 structure ValidatedProgram where
   length : Nat
   instructions : Vector (ValidatedInstruction length) length
-  deriving Repr
+  deriving DecidableEq, Repr
 
 namespace ValidatedProgram
 
